\documentclass{article}
		
\usepackage{amssymb}
\usepackage{amsmath}
\usepackage[margin=1 in]{geometry}

\usepackage{tabularx}
\usepackage{bbm}

\usepackage{fancyhdr}
\pagestyle{fancy}
\lhead{Markov Decision Theory}
\rhead{John Gilbertson}

%\usepackage[backend=bibtex,style=numeric,sorting=none]{biblatex}
%\addbibresource{bibliography.bib}

\title{Markov Decision Theory}
\author{John Gilbertson}
\date{\today}

\begin{document}

\maketitle

\tableofcontents

\newpage

\section{Aim}

Immediately after a patient arrives and begins waiting for service, want to decide when the next patient should be scheduled to arrive given the current state.

\section{Assumptions}

\begin{itemize}
	\item Patients can be scheduled at any future (or present) time
	\item Patients are punctual and arrive when scheduled
	\item iid exponential service times with mean $\mu$ and single server
\end{itemize}

\section{Parameters}

\begin{tabularx}{\textwidth}{c c X}
	$N$ & : & number of patients remaining to be scheduled \\
	$k$ & : & current number of patients in queue (i.e., the current state) \\
	$j$ & : & number of patients in queue immediately after the next patient arrives (i.e., the next state) \\
	$a$ & : & time next patient is scheduled to arrive (relative to current time) \\
	$C_{N} (k)$ & : & expected cost of being in state $k$ with $N$ patients still to be scheduled \\
	$p_{a} (k, j)$ & : & probability of transitioning from state $k$ to state $j$ over the time interval $a$ \\
	$R_{a} (k, j)$ & : & expected cost of transitioning from state $k$ to state $j$ over the time interval $a$ \\
\end{tabularx}

\section{Optimal Policy}

The optimal policy is the $a^{*}$ given by the following equation (for $N \geq 1$):

\begin{equation}
	C_{N} (k) = \min_{a \geq 0} \left[ \sum_{j = 1}^{k + 1} p_{a} (k, j) \Big( R_{a} (k, j) + C_{N - 1} (j) \Big) \right]
\end{equation}

\section{Calculations}

\subsection{None Remaining to be Scheduled}

\subsubsection{Expected Waiting Time}

Let $w_{i}$ be the expected waiting time of the patient that is currently in position $i$ in the queue

\begin{equation*}
	w_{i} = \mu i
\end{equation*}

\subsubsection{Expected Waiting Cost}

Let $c_{W}$ be the waiting cost of each patient

\begin{align*}
	C_{0} (k) & = c_{W} \sum_{i = 1}^{k} w_{i} \\
	& = c_{W} \mu \sum_{i = 1}^{k} i \\
	C_{0} (k) & = \frac{c_{W} \mu k (k + 1)}{2} \\
\end{align*}

\subsection{Erlang Distribution}

\begin{itemize}
	\item Let $S_{i}$ be the service time of the patient that is currently in position $i$ in the queue
	\item $S_{1}, \ldots, S_{k}$ are iid Exp$(\mu)$
	\item $X = \sum_{i = 1}^{k} S_{i}$ is the total service time of the $k$ patients
	\item $X \sim \text{Erlang} (k, \mu)$ such that for $x > 0$:
		\begin{equation*}
			f (x; k, \mu) = \frac{1}{\mu \cdot (k - 1)!} \left( \frac{x}{\mu} \right)^{k - 1} \exp \left[ \frac{-x}{\mu} \right]
		\end{equation*}
\end{itemize}

\subsubsection{Cumulative Distribution Function}

\begin{itemize}
	\item The number of patients served by the health care system from time 0 to time $t$ is a poisson point process $W_{t} \sim \text{Poisson} \left( \frac{t}{\mu} \right)$
	\item $\{ X > a \}$ and $\{ W_{a} < k \}$ are both the events that not all of the $k$ patients are served from time 0 to time $a$ such that $\mathbb{P} (X > a) = \mathbb{P} (W_{a} < k)$
\end{itemize}

\begin{align*}
	F (a; k, \mu) & = \mathbb{P} (X \leq a) \\
	& = 1 - \mathbb{P} (X > a) \\
	& = 1 - \mathbb{P} (W_{a} < k) \\
	& = 1 - \sum_{n = 0}^{k - 1} \mathbb{P} (W_{a} = n) \\
	F (a; k, \mu) & = 1 - \sum_{n = 0}^{k - 1} \frac{1}{n!} \left( \frac{a}{\mu} \right)^{n} \exp \left[ \frac{-a}{\mu} \right] \\
\end{align*}

\subsubsection{Conditional Expectation}

\begin{align*}
	G (a; k, \mu) & = \mathbb{E} [X | X \leq a] \\
	& = \int x \cdot \mathbb{P} (X \in dx | X \leq a) \\
	& = \int x \cdot \frac{\mathbb{P} (X \in dx, X \leq a)}{\mathbb{P} (X \leq a)} \\
	& = \frac{1}{F (a; k, \mu)} \int_{0}^{a} x \cdot f (x; k, \mu) d x \\
	& = \frac{1}{F (a; k, \mu)} \int_{0}^{a} x \cdot \frac{1}{\mu \cdot (k - 1)!} \left( \frac{x}{\mu} \right)^{k - 1} \exp \left[ \frac{-x}{\mu} \right] d x \\
	& = \frac{\mu k}{F (a; k, \mu)} \int_{0}^{a} \frac{1}{\mu \cdot k!} \left( \frac{x}{\mu} \right)^{k} \exp \left[ \frac{-x}{\mu} \right] d x \\
	& = \frac{\mu k}{F (a; k, \mu)} \int_{0}^{a} f (x; k + 1, \mu) d x \\
	G (a; k, \mu) & = \mu k \cdot \frac{F (a; k + 1, \mu)}{F (a; k, \mu)} \\
\end{align*}

\subsection{Probability of Transition}

\subsubsection{Case 1 $a = 0$}

\begin{equation*}
	p_{a} (k, j) = \mathbbm{1} (j = k + 1) \\
\end{equation*}

\subsubsection{Case 2 $a > 0, k = 0$}

\begin{equation*}
	p_{a} (k, j) = \mathbbm{1} (j = 1) \\
\end{equation*}

\subsubsection{Case 3 $a > 0, k \geq 1, j = 1$}

\begin{align*}
	p_{a} (k, j) & = \mathbb{P} \left( \sum_{i = 1}^{k} S_{i} \leq a \right) \\
	p_{a} (k, j) & = F (a; k, \mu) \\
\end{align*}

\subsubsection{Case 4 $a > 0, k \geq 1, 2 \leq j \leq k$}

\begin{align*}
	p_{a} (k, j) & = \mathbb{P} \left( \sum_{i = 1}^{k - (j - 1)} S_{i} \leq a, \sum_{i = 1}^{k - (j - 1) + 1} S_{i} > a \right) \\
	& = \mathbb{P} \left( \sum_{i = 1}^{k - (j - 1)} S_{i} \leq a, \sum_{i = 1}^{k - (j - 1)} S_{i} + S_{k - (j - 1) + 1} > a \right) \\
	& = \mathbb{P} \left( \sum_{i = 1}^{k - (j - 1)} S_{i} \leq a, S_{k - (j - 1) + 1} > a - \sum_{i = 1}^{k - (j - 1)} S_{i} \right) \\
	& = \int \mathbb{P} \left( \sum_{i = 1}^{k - (j - 1)} S_{i} \leq a, S_{k - (j - 1) + 1} > a - \sum_{i = 1}^{k - (j - 1)} S_{i} \ \vline \ \sum_{i = 1}^{k - (j - 1)} S_{i} = z \right) \mathbb{P} \left( \sum_{i = 1}^{k - (j - 1)} S_{i} \in d z \right) \\
	& = \int_{0}^{\infty} \mathbb{P} \left( z \leq a, S_{k - (j - 1) + 1} > a - z \right) f (z; k - (j - 1), \mu) d z \\
	& = \int_{0}^{a} \mathbb{P} \left( S_{k - (j - 1) + 1} > a - z \right) f (z; k - (j - 1), \mu) d z \\
	& = \int_{0}^{a} f (z; k - (j - 1), \mu) \Big( 1 - \mathbb{P} (S_{k - ( j - 1) + 1} \leq a - z) \Big) d z \\
	& = \int_{0}^{a} f (z; k - (j - 1), \mu) \Big( 1 - \mathbb{P} (S_{1} \leq a - z) \Big) d z \\
	& = \int_{0}^{a} f (z; k - (j - 1), \mu) \Big( 1 - F (a - z; 1, \mu) \Big) d z \\
	& = \int_{0}^{a} \frac{1}{\mu \cdot (k - (j - 1) - 1)!} \left( \frac{z}{\mu} \right)^{k - (j - 1) - 1} \exp \left[ \frac{-z}{\mu} \right] \exp \left[ \frac{- (a - z)}{\mu} \right] d z \\
	& = \frac{1}{(k - (j - 1) - 1)!} \left( \frac{1}{\mu} \right)^{k - (j - 1)} \exp \left[ \frac{-a}{\mu} \right] \int_{0}^{a} z^{k - (j - 1) - 1} d z \\
	p_{a} (k, j) & = \frac{1}{(k - (j - 1) - 1)!} \left( \frac{1}{\mu} \right)^{k - (j - 1)} \exp \left[ \frac{-a}{\mu} \right] \left[ \frac{z^{k - (j - 1)}}{k - (j - 1)} \right]_{z = 0}^{z = a} \\
\end{align*}

\begin{align*}
	p_{a} (k, j) & = \frac{1}{(k - (j - 1))!} \left( \frac{a}{\mu} \right)^{k - (j - 1)} \exp \left[ \frac{-a}{\mu} \right] \\
	& = \left[ 1 - \sum_{n = 0}^{k - (j - 1) - 1} \frac{1}{n!} \left( \frac{a}{\mu} \right)^{n} \exp \left[ \frac{-a}{\mu} \right] \right] - \left[ 1 - \sum_{n = 0}^{k - (j - 1)} \frac{1}{n!} \left( \frac{a}{\mu} \right)^{n} \exp \left[ \frac{-a}{\mu} \right] \right] \\
	p_{a} (k, j) & = F \Big( a; k - (j - 1) - 1, \mu \Big) - F \Big( a; k - (j - 1), \mu \Big) \\
\end{align*}

\subsubsection{Case 5 $a > 0, k \geq 1, j = (k + 1)$}

\begin{align*}
	p_{a} (k, j) & = \mathbb{P} (S_{1} > a) \\
	& = 1 - \mathbb{P} (S_{1} \leq a) \\
	p_{a} (k, j) & = 1 - F (a; 1, \mu) \\
\end{align*}

\subsubsection{All Other Cases}

\begin{equation*}
	p_{a} (i, j) = 0 \\
\end{equation*}

\subsubsection{Summary}

These results can be summarised as:

\begin{equation}
	p_{a} (k, j) = \begin{cases} \mathbbm{1} (j = k + 1) & \text{where $a = 0$} \\
						\mathbbm{1} (j = 1) & \text{where $a > 0$, $k = 0$} \\
						F (a; k, \mu) & \text{where $a > 0$, $k \geq 1$, $j = 1$} \\
						F \big( a; k - (j - 1) - 1, \mu \big) - F \big( a; k - (j - 1), \mu \big) & \text{where $a > 0$, $k \geq 1$, $2 \leq j \leq k$} \\
						1 - F (a; 1, \mu) & \text{where $a > 0$, $k \geq 1$, $j = (k + 1)$} \\
						0 & \text{otherwise} \end{cases}
\end{equation}

\subsection{Expected Cost of Transition}

\subsubsection{Case 1 $a = 0$}

\begin{equation*}
	R_{a} (k, j) = 0 \\
\end{equation*}

\subsubsection{Case 2 $a > 0, k = 0$}

Let $c_{I}$ be the cost of the doctor's idle time

\begin{equation*}
	R_{a} (k, j) = c_{I} a \\
\end{equation*}

\subsubsection{Case 3 $a > 0, k \geq 1, j = 1$}

\begin{align*}
	R_{a} (k, j) & = \sum_{i = 1}^{k} c_{W} \mathbb{E} \left[ \sum_{l = 1}^{i} S_{l} \ \vline \ \sum_{n = 1}^{k} S_{n} \leq a \right] + c_{I} \mathbb{E} \left[ a - \sum_{n = 1}^{k} S_{n} \ \vline \ \sum_{n = 1}^{k} S_{n} \leq a \right] \\
	& = c_{W} \sum_{i = 1}^{k} \sum_{l = 1}^{i} \mathbb{E} \left[ S_{l} \ \vline \ \sum_{n = 1}^{k} S_{n} \leq a \right] + c_{I} a - c_{I} \mathbb{E} \left[ \sum_{n = 1}^{k} S_{n} \ \vline \ \sum_{n = 1}^{k} S_{n} \leq a \right] \\
	& = c_{W} \mathbb{E} \left[ S_{1} \ \vline \ \sum_{n = 1}^{k} S_{n} \leq a \right] \sum_{i = 1}^{k} i + c_{I} a - c_{I} G (a; k, \mu) \\
	& = \frac{c_{W} k (k + 1)}{2} \mathbb{E} \left[ S_{1} \ \vline \ \sum_{n = 1}^{k} S_{n} \leq a \right] + c_{I} a - c_{I} G (a; k, \mu) \\
	& = \frac{c_{W} (k + 1)}{2} \mathbb{E} \left[ \sum_{n = 1}^{k} S_{n} \ \vline \ \sum_{n = 1}^{k} S_{n} \leq a \right] + c_{I} a - c_{I} G (a; k, \mu) \\
	& = c_{I} a + \frac{c_{W} G (a; k, \mu) (k + 1)}{2} - c_{I} G (a; k, \mu) \\
	R_{a} (k, j) & = c_{I} a + \frac{G (a; k, \mu) \Big( c_{W} (k + 1) - 2 c_{I} \Big)}{2} \\
\end{align*}

\subsubsection{Case 4 $a > 0, k \geq 1, 2 \leq j \leq k$}

\begin{align*}
	R_{a} (k, j) & = c_{W} a (j - 1) + \sum_{i = 1}^{k - (j - 1)} c_{W} \mathbb{E} \left[ \sum_{l = 1}^{i} S_{l} \ \vline \ \sum_{n = 1}^{k - (j - 1)} S_{n} \leq a \right] \\
	& = c_{W} a (j - 1) + c_{W} \sum_{i = 1}^{k - (j - 1)} \sum_{l = 1}^{i} \mathbb{E} \left[ S_{l} \ \vline \ \sum_{n = 1}^{k - (j - 1)} S_{n} \leq a \right] \\
	& = c_{W} a (j - 1) + c_{W} \mathbb{E} \left[ S_{1} \ \vline \ \sum_{n = 1}^{k - (j - 1)} S_{n} \leq a \right] \sum_{i = 1}^{k - (j - 1)} i \\
	& = c_{W} a (j - 1) + \frac{c_{W} \Big( k - (j - 1) \Big) \Big( k - (j - 1) + 1 \Big)}{2} \mathbb{E} \left[ S_{1} \ \vline \ \sum_{n = 1}^{k - (j - 1)} S_{n} \leq a \right] \\
	& = c_{W} a (j - 1) + \frac{c_{W} \Big( k - (j - 1) + 1 \Big)}{2} \mathbb{E} \left[ \sum_{n = 1}^{k - (j - 1)} S_{n} \ \vline \ \sum_{n = 1}^{k - (j - 1)} S_{n} \leq a \right] \\
	R_{a} (k, j) & = c_{W} a (j - 1) + \frac{c_{W} G \Big( a; k - (j - 1), \mu \Big) \Big( k - (j - 1) + 1 \Big)}{2} \\
\end{align*}

\subsubsection{Case 5 $a > 0, k \geq 1, j = (k + 1)$}

\begin{equation*}
	R_{a} (k, j) = c_{W} a k \\
\end{equation*}

\newpage

\subsubsection{Summary}

These results can be summarised as:

\begin{equation}
	R_{a} (k, j) = \begin{cases} 0 & \text{where $a = 0$} \\
						c_{I} a + \frac{G (a; k, \mu) \big( c_{w} (k + 1) - 2 c_{I} \big)}{2} & \text{where $a > 0$, $k \geq 0$, $j = 1$} \\
						c_{W} a (j - 1) + \frac{c_{W} G \big( a; k - (j - 1), \mu \big) \big( k - (j - 1) + 1 \big)}{2} & \text{where $a > 0$, $k \geq 1$, $2 \leq j \leq (k + 1)$} \end{cases}
\end{equation}

\end{document}






























